Tests/AxiomAudit.lean
@@ -173,6 +173,7 @@ elab "#assert_axioms " id:ident : command => do
 /-! ## Consensus: transaction premises -/
 
 #assert_axioms BtcVerified.Tx.isWellFormed_iff
+#assert_axioms BtcVerified.Tx.coinbaseWellFormed_iff
 #assert_axioms BtcVerified.Tx.strippedSize_bound_iff_core
 #assert_axioms BtcVerified.Tx.WellFormed.outputs_length_le
 #assert_axioms BtcVerified.Coin.isMature_iff
